tests/hashmap/Hashmap.Properties.fsti
@@ -1,0 +1,214 @@
+(** Properties about the hashmap *)
+module Hashmap.Properties
+open Primitives
+open FStar.List.Tot
+open FStar.Mul
+open Hashmap.Types
+open Hashmap.Clauses
+open Hashmap.Funs
+
+#set-options "--z3rlimit 50 --fuel 0 --ifuel 1"
+
+// Small trick to align the .fst and the .fsti
+val _align_fsti : unit
+
+(*** Utilities *)
+
+type key : eqtype = usize
+
+type hash : eqtype = usize
+
+val hash_map_t_inv (#t : Type0) (hm : hash_map_t t) : Type0
+
+val len_s (#t : Type0) (hm : hash_map_t t) : nat
+
+val find_s (#t : Type0) (hm : hash_map_t t) (k : key) : option t
+
+(*** new *)
+
+/// [new] doesn't fail and returns an empty hash map
+val hash_map_new_fwd_lem (t : Type0) :
+  Lemma
+  (ensures (
+    match hash_map_new_fwd t with
+    | Fail -> False
+    | Return hm ->
+      // The hash map invariant is satisfied
+      hash_map_t_inv hm /\
+      // The hash map has a length of 0
+      len_s hm = 0 /\
+      // It contains no bindings
+      (forall k. find_s hm k == None)))
+
+(*** [clear] *)
+
+/// [clear] doesn't fail and turns the hash map into an empty map
+val hash_map_clear_fwd_back_lem
+  (#t : Type0) (self : hash_map_t t) :
+  Lemma
+  (requires (hash_map_t_inv self))
+  (ensures (
+    match hash_map_clear_fwd_back t self with
+    | Fail -> False
+    | Return hm ->
+      // The hash map invariant is satisfied
+      hash_map_t_inv hm /\
+      // The hash map has a length of 0
+      len_s hm = 0 /\
+      // It contains no bindings
+      (forall k. find_s hm k == None)))
+
+(*** [len] *)
+
+/// [len] can't fail and returns the length (the number of elements) of the hash map
+val hash_map_len_fwd_lem (#t : Type0) (self : hash_map_t t) :
+  Lemma
+  (requires (hash_map_t_inv self))
+  (ensures (
+    match hash_map_len_fwd t self with
+    | Fail -> False
+    | Return l -> l = len_s self))
+
+
+(*** [insert'fwd_back] *)
+
+/// The backward function for [insert] (note it is named "...'fwd_back" because
+/// the forward function doesn't return anything, and is was thus filtered - in a
+/// sense the effect of applying the forward function then the backward function is
+/// entirely given by the backward function alone).
+/// [insert'fwd_back] simply inserts a binding.
+val hash_map_insert_fwd_back_lem
+  (#t : Type0) (self : hash_map_t t) (key : usize) (value : t) :
+  Lemma
+  (requires (hash_map_t_inv self))
+  (ensures (
+    match hash_map_insert_fwd_back t self key value with
+    | Fail ->
+      // We can fail only if:
+      // - the key is not in the map and we thus need to add it
+      None? (find_s self key) /\
+      // - and we are already saturated (we can't increment the internal counter)
+      len_s self = usize_max
+    | Return hm' ->
+      // The invariant is preserved
+      hash_map_t_inv hm' /\
+      // [key] maps to [value]
+      find_s hm' key == Some value /\
+      // The other bindings are preserved
+      (forall k'. k' <> key ==> find_s hm' k' == find_s self k') /\
+      begin
+      // The length is incremented, iff we inserted a new key
+      match find_s self key with
+      | None -> len_s hm' = len_s self + 1
+      | Some _ -> len_s hm' = len_s self
+      end))
+
+
+(*** [contains_key] *)
+
+/// [contains_key'fwd] can't fail and return `true` if and only if there is
+/// a binding for key [key]
+val hash_map_contains_key_fwd_lem
+  (#t : Type0) (self : hash_map_t t) (key : usize) :
+  Lemma
+  (requires (hash_map_t_inv self))
+  (ensures (
+    match hash_map_contains_key_fwd t self key with
+    | Fail -> False
+    | Return b -> b = Some? (find_s self key)))
+
+(*** [get'fwd] *)
+
+/// [get] returns (a shared borrow to) the binding for key [key]
+val hash_map_get_fwd_lem
+  (#t : Type0) (self : hash_map_t t) (key : usize) :
+  Lemma
+  (requires (hash_map_t_inv self))
+  (ensures (
+    match hash_map_get_fwd t self key, find_s self key with
+    | Fail, None -> True
+    | Return x, Some x' -> x == x'
+    | _ -> False))
+
+(*** [get_mut'fwd] *)
+
+/// [get_mut'fwd] returns (mutable borrows to) the binding for key [key].
+val hash_map_get_mut_fwd_lem
+  (#t : Type0) (self : hash_map_t t) (key : usize) :
+  Lemma
+  (requires (hash_map_t_inv self))
+  (ensures (
+    match hash_map_get_mut_fwd t self key, find_s self key with
+    | Fail, None -> True
+    | Return x, Some x' -> x == x'
+    | _ -> False))
+
+
+(*** [get_mut'back] *)
+
+/// [get_mut'back] updates the binding for key [key], without failing.
+/// A call to [get_mut'back] must follow a call to [get_mut'fwd], which gives
+/// us that there must be a binding for key [key] in the map (otherwise we
+/// can't prove the absence of failure).
+val hash_map_get_mut_back_lem
+  (#t : Type0) (hm : hash_map_t t) (key : usize) (ret : t) :
+  Lemma
+  (requires (
+    hash_map_t_inv hm /\
+    // A call to the backward function must follow a call to the forward
+    // function, whose success gives us that there is a binding for the key.
+    Some? (find_s hm key)))
+  (ensures (
+    match hash_map_get_mut_back t hm key ret with
+    | Fail -> False // Can't fail
+    | Return hm' ->
+     // The invariant is preserved
+     hash_map_t_inv hm' /\
+     // The length is preserved
+     len_s hm' = len_s hm /\
+     // [key] maps to the update value, [ret]
+     find_s hm' key == Some ret /\
+     // The other bindings are preserved
+     (forall k'. k' <> key ==> find_s hm' k' == find_s hm k')))
+
+(*** [remove'fwd] *)
+
+/// [remove'fwd] returns the (optional) element which has been removed from the map
+/// (the rust function *moves* it out of the map).
+val hash_map_remove_fwd_lem
+  (#t : Type0) (self : hash_map_t t) (key : usize) :
+  Lemma
+  (requires (hash_map_t_inv self))
+  (ensures (
+    match hash_map_remove_fwd t self key with
+    | Fail -> False
+    | Return opt_x -> opt_x == find_s self key))
+
+
+(*** [remove'back] *)
+
+/// The hash map given as parameter to [remove] is given through a mutable borrow:
+/// hence the backward function which gives back the updated map, without the
+/// binding.
+val hash_map_remove_back_lem
+  (#t : Type0) (self : hash_map_t t) (key : usize) :
+  Lemma
+  (requires (hash_map_t_inv self))
+  (ensures (
+    match hash_map_remove_back t self key with
+    | Fail -> False
+    | Return hm' ->
+      // The invariant is preserved
+      hash_map_t_inv self /\
+      // The binding for [key] is not there anymore
+      find_s hm' key == None /\
+      // The other bindings are preserved
+      (forall k'. k' <> key ==> find_s hm' k' == find_s self k') /\
+      begin
+      // The length is decremented iff the key was in the map
+      let len = len_s self in
+      let len' = len_s hm' in
+      match find_s self key with
+      | None -> len = len'
+      | Some _ -> len = len' + 1
+      end))
